txn-data-consistency/EP+_TCCv_update_kv_invs.thy
@@ -75,19 +75,137 @@ lemma not_last_version_not_read:
   using assms
   apply (auto simp add: ) oops
 
+definition Rtxn_Once_in_rs' where
+  "Rtxn_Once_in_rs' s k \<longleftrightarrow> (\<forall>t.
+    (\<forall>t' cts v rs deps. svr_state (svrs s k) t' = Commit cts v rs deps \<longrightarrow> t \<notin> rs) \<or> 
+    (\<exists>!t'. \<exists>cts v rs deps. svr_state (svrs s k) t' = Commit cts v rs deps \<and> t \<in> rs))"
+
+inductive ver_grows :: "'v ver_state \<Rightarrow> 'v ver_state \<Rightarrow> bool" (infix "\<sqsubseteq>\<^sub>v" 60) where
+  "ver_grows v v" |
+  "ver_grows No_Ver (Prep pts v)" |
+  "ver_grows No_Ver (Commit cts v rs deps)" |
+  "ver_grows (Prep pts v) (Commit cts v rs deps)" |
+  "rs \<subseteq> rs' \<Longrightarrow> ver_grows (Commit cts v rs deps) (Commit cts v rs' deps)"
+
+lemma ver_grows_inv:
+  assumes "state_trans s e s'"
+  shows "\<forall>t. svr_state (svrs s k) t \<sqsubseteq>\<^sub>v svr_state (svrs s' k) t"
+  using assms
+proof (induction e)
+  case (RegR x1 x2 x3 x4)
+  then show ?case by (auto simp add: tps_trans_defs add_to_readerset_def
+   intro: ver_grows.intros split: ver_state.split)
+next
+  case (CommitW x1 x2 x3 x4 x5)
+  then show ?case apply (auto simp add: tps_trans_defs intro: ver_grows.intros)
+    by (metis is_prepared.elims(2) ver_grows.intros(4) ver_state.sel(3))
+qed (auto simp add: tps_trans_defs intro: ver_grows.intros)
+
+inductive committed_ver_grows :: "'v ver_state \<Rightarrow> 'v ver_state \<Rightarrow> bool" (infix "\<sqsubseteq>\<^sub>c\<^sub>v" 60) where
+  "committed_ver_grows v v" |
+  "rs \<subseteq> rs' \<Longrightarrow> committed_ver_grows (Commit cts v rs deps) (Commit cts v rs' deps)"
+
+lemma rtxn_committed_ver_grows:
+  assumes "state_trans s e s'"
+    and "\<forall>k t v. e \<noteq> PrepW k t v"
+    and "\<forall>k t v cts deps. e \<noteq> CommitW k t v cts deps"
+  shows "committed_ver_grows (svr_state (svrs s k) t) (svr_state (svrs s' k) t)"
+  using assms
+proof (induction e)
+  case (RegR x1 x2 x3 x4)
+  then show ?case by (auto simp add: tps_trans_defs add_to_readerset_def
+   intro: committed_ver_grows.intros split: ver_state.split)
+qed (auto simp add: tps_trans_defs intro: committed_ver_grows.intros)
+
+lemma rtxn_get_ctx:
+  assumes "state_trans s e s'"
+    and "\<forall>k t v. e \<noteq> PrepW k t v"
+    and "\<forall>k t v cts deps. e \<noteq> CommitW k t v cts deps"
+  shows "get_ctx s' kvt_map = get_ctx s kvt_map"
+  using assms
+  apply (auto simp add: get_ctx_def)
+  apply (smt (verit) committed_ver_grows.cases insertCI rtxn_committed_ver_grows ver_state.inject(2))
+  apply (smt (verit) committed_ver_grows.simps insert_iff rtxn_committed_ver_grows ver_state.inject(2))
+  apply (smt (verit) committed_ver_grows.simps insertCI rtxn_committed_ver_grows ver_state.inject(2))
+  by (smt (verit) committed_ver_grows.simps insert_iff rtxn_committed_ver_grows ver_state.inject(2))
+
+lemma rtxn_get_ctx_pres:
+  assumes "\<And>k t. ver_grows (svr_state (svrs s k) t) (svr_state (svrs s' k) t)"
+  shows "get_ctx s' kvt_map = get_ctx s kvt_map"
+  using assms
+  oops
+  
+
+definition Rtxn_Once_in_rs where
+  "Rtxn_Once_in_rs s cl \<longleftrightarrow> (\<forall>k t_wr cts v rs deps. 
+    svr_state (svrs s k) t_wr = Commit cts v rs deps \<and> get_txn s cl \<in> rs \<longrightarrow>
+    (\<exists>keys kvt_map. cl_state (cls s cl) = RtxnInProg keys kvt_map \<and>
+    t_wr = commit_order s k ! Max (view_of (commit_order s) (cl_ctx (cls s cl) \<union> get_ctx s kvt_map) k)))"
+
+lemmas Rtxn_Once_in_rsI = Rtxn_Once_in_rs_def[THEN iffD2, rule_format]
+lemmas Rtxn_Once_in_rsE[elim] = Rtxn_Once_in_rs_def[THEN iffD1, elim_format, rule_format]
+
+lemma reach_rtxn_once_in_rs [simp]: "reach tps s \<Longrightarrow> Rtxn_Once_in_rs s cl"
+proof(induction s rule: reach.induct)
+  case (reach_init s)
+  then show ?case
+    by (auto simp add: Rtxn_Once_in_rs_def tps_defs split: if_split_asm)
+next
+  case (reach_trans s e s')
+  then show ?case using rtxn_get_ctx[of s e s']
+  proof (induction)
+    case (RInvoke x1 x2)
+    then show ?case apply (auto simp add: Rtxn_Once_in_rs_def tps_trans_defs)
+      by blast
+  next
+    case (Read x1 x2 x3 x4)
+    then show ?case apply (auto simp add: Rtxn_Once_in_rs_def tps_trans_defs) sorry
+  next
+    case (RDone x1 x2 x3 x4)
+    then show ?case apply (auto simp add: Rtxn_Once_in_rs_def tps_trans_defs)
+      using FTid_notin_rs_def by blast
+  next
+    case (WInvoke x1 x2)
+    then show ?case apply (simp add: Rtxn_Once_in_rs_def tps_trans_defs)
+      by (metis txn_state.distinct(1))
+  next
+    case (WCommit x1 x2 x3 x4 x5)
+    then show ?case apply (simp add: Rtxn_Once_in_rs_def tps_trans_defs) sorry
+  next
+    case (WDone x1 x2)
+    then show ?case apply (auto simp add: Rtxn_Once_in_rs_def tps_trans_defs)
+      using FTid_notin_rs_def by blast
+  next
+    case (RegR x1 x2 x3 x4)
+    then show ?case apply (auto simp add: Rtxn_Once_in_rs_def tps_trans_defs)
+      subgoal for t_wr keys kvt_map cts v rs deps
+        apply (cases "cl = get_cl x2", simp_all)
+        apply (cases "cl_state (cls s cl)", simp_all)
+      subgoal for keys'
+        using Fresh_wr_notin_rs_def[of s "get_cl x2"]
+        add_to_readerset_commit_subset[of "svr_state (svrs s x1)" x2
+         "read_at (svr_state (svrs s x1)) (gst (cls s (get_cl x2))) (get_cl x2)" t_wr cts v rs deps]
+        apply auto sorry sorry sorry
+  next
+    case (PrepW x1 x2 x3)
+    then show ?case apply (simp add: Rtxn_Once_in_rs_def tps_trans_defs) sorry
+  next
+    case (CommitW x1 x2 x3 x4 x5)
+    then show ?case apply (simp add: Rtxn_Once_in_rs_def tps_trans_defs) sorry
+  qed simp
+qed
+
 lemma read_done_kvs_of_s:
   assumes "read_done cl kvt_map sn u'' s s'"
     and "cl_state (cls s cl) = RtxnInProg (dom kvt_map) kvt_map"
     and "\<forall>k. commit_order s' k = commit_order s k"
     and "\<forall>k. CO_Distinct s k"
-    and "\<forall>k. CO_not_No_Ver s k"
     and "\<forall>k. Cl_Ctx_Sub_CO s k"
     and "\<forall>k. Get_Ctx_Sub_CO s k"
     and "\<forall>k. T0_in_CO s k"
     and "View_Init s cl"
     and "Rtxn_IdleK_notin_rs s cl"
-    and "Rtxn_RegK_in_rs s cl"
-    and "Kvt_map_t_Committed s cl"
+    and "\<And>k. Rtxn_Once_in_rs s k"
     and "Ctx_Committed s"
     and "Deps_Committed s"
   shows "kvs_of_s s' = update_kv (Tn_cl sn cl)
@@ -95,17 +213,18 @@ lemma read_done_kvs_of_s:
           (view_of (commit_order s) (cl_ctx (cls s cl) \<union> get_ctx s kvt_map))
           (kvs_of_s s)"
   using assms
-  apply (auto simp add: update_kv_defs update_kv_writes_def update_kv_key_reads_def)
-  apply (rule ext) apply (auto split: option.split)
+  apply (auto simp add: update_kv_defs)
+  apply (rule ext) subgoal for k apply (cases "map_option fst (kvt_map k)")
   subgoal apply (auto simp add: read_done_def kvs_of_s_defs split: ver_state.split)
     by (smt (verit, best) Rtxn_IdleK_notin_rs_def domIff less_antisym txid0.collapse)
-  subgoal for k v t_wr
-    apply (auto simp add: Let_def last_version_def kvs_of_s_def)
+  subgoal for v
+    apply (auto simp add: Let_def kvs_of_s_def)
     apply (subst map_list_update)
     subgoal by (meson Max_in ctx_get_ctx_subset_co finite_view_of view_of_in_range view_of_non_emp)
     subgoal by blast
-    subgoal apply (auto simp add: txn_to_vers_def)
-      subgoal using Max_view_of_in_range[of s "cl_ctx (cls s cl) \<union> get_ctx s kvt_map" k]
+    subgoal for t_wr apply (auto simp add: txn_to_vers_def)
+        subgoal \<comment> \<open>t_wr' = commit_order ! Max (view_of ...)\<close>
+          using Max_view_of_in_range[of s "cl_ctx (cls s cl) \<union> get_ctx s kvt_map" k]
             view_of_committed[of s cl "dom kvt_map" kvt_map k 
           "Max (view_of (commit_order s) (cl_ctx (cls s cl) \<union> get_ctx s kvt_map) k)"]
           ctx_get_ctx_subset_co[of s cl "dom kvt_map" kvt_map k]
@@ -115,11 +234,13 @@ lemma read_done_kvs_of_s:
          (*apply (auto simp add: read_done_def split: ver_state.split)
          apply (metis not_less_less_Suc_eq txid0.exhaust_sel)
         using Rtxn_RegK_in_rs_def[of s] Kvt_map_t_Committed_def[of s]*) sorry
-       subgoal for t_wr' using CO_not_No_Ver_def [of s k]
+        subgoal for t_wr' \<comment> \<open>t_wr' \<noteq> commit_order ! Max (view_of ...)\<close>
          apply (auto simp add: read_done_def split: ver_state.split)
-         subgoal for cts' v' rs' deps' t_rd
-           apply (cases "get_sn t_rd = cl_sn (cls s (get_cl t_rd))", simp_all)
-           apply (cases t_rd, auto) sorry
-         . . . .
+          subgoal for cts' v' rs' deps' t_rd
+           apply (cases "get_sn t_rd = cl_sn (cls s cl)", simp_all)
+           apply (cases t_rd, auto)
+           using Rtxn_Once_in_rs_def by (smt (z3) txn_state.inject(1)).
+       done.
+     done.
 
 end
